proof/Simple/EvJudge.v
@@ -10,34 +10,33 @@ Require Export Exp.
    This is also called 'Natural Semantics'.
  *)
 Inductive EVAL : exp -> exp -> Prop :=
- | EVValue
+ | EVDone
    :  forall v2
-   ,  value v2
-   -> EVAL v2 v2
+   ,  whnfX  v2
+   -> EVAL   v2 v2
 
  | EVLamApp
    :  forall x1 t11 x12 x2 v2 v3
-   ,                              value v2               -> value v3
-   -> EVAL x1 (XLam t11 x12) -> EVAL x2 v2 -> EVAL (subst v2 x12) v3
+   ,  EVAL x1 (XLam t11 x12) -> EVAL x2 v2 -> EVAL (subst v2 x12) v3
    -> EVAL (XApp x1 x2) v3.
 
 Hint Constructors EVAL.
 
 
-(* A terminating big-step evaluation always produces a value.
+(* A terminating big-step evaluation always produces a whnf.
    The fact that the evaluation has terminated is implied by the fact
    that we have a proof of EVAL to pass to this lemma. If the
    evaluation was non-terminating, then we wouldn't have a finite
    proof of EVAL.
  *)
-Lemma eval_produces_value
+Lemma eval_produces_whnfX
  :  forall x1 v1
- ,  EVAL x1 v1
- -> value v1.
+ ,  EVAL   x1 v1
+ -> whnfX  v1.
 Proof.
- intros. destruct H; auto.
+ intros. induction H; eauto.
 Qed.
-Hint Resolve eval_produces_value.
+Hint Resolve eval_produces_whnfX.
 
 
 (* Big to Small steps ***********************************************)
@@ -57,16 +56,23 @@ Proof.
  Case "EVLamApp".
   intros. inverts HT.
 
-  lets E1: IHHE1 H4. clear IHHE1. destruct E1 as [n1].
-  lets E2: IHHE2 H6. clear IHHE2. destruct E2 as [n2].
+  lets E1: IHHE1 H2. clear IHHE1. destruct E1 as [n1].
+  lets E2: IHHE2 H4. clear IHHE2. destruct E2 as [n2].
 
-  lets T1: preservation_steps H4 H1. inverts keep T1.
-  lets T2: preservation_steps H6 H2.
-  lets T3: subst_value_value H7 T2.
+  lets T1: preservation_steps H2 H. inverts keep T1.
+  lets T2: preservation_steps H4 H0.
+  lets T3: subst_value_value H5 T2.
   lets E3: IHHE3 T3. clear IHHE3. destruct E3 as [n3].
 
   exists (n1 + (n2 + (1 + n3))).
-   repeat (try (eapply ESLink); eauto).
+   eapply ESLink.
+    eapply steps_app1. eauto.
+   eapply ESLink.
+    eapply steps_app2. eauto. eauto.
+   eapply ESLink.
+    eapply ESStep.
+     eapply ESLamApp. eauto.
+   eauto.      
 Qed.
 
 
@@ -83,30 +89,18 @@ Proof.
  eapply EVLamApp.
   eauto. eauto.
   inverts H0. 
-  apply EVValue.
-   skip.         (* XLam t11 x12 isn't ness a value. We prob
-                    want whnf in the eval judgement instead of value *)
+  apply EVDone.
+   inverts H. auto.
    eauto.
-   auto.
-
+ 
  Case "x1 steps".
   inverts H. inverts H1.
    inverts H.
-   eapply EVLamApp.
-    apply H3.
-    auto.
-    eapply IHSTEP; eauto.
-    eauto.
-    eauto.
+   eapply EVLamApp; eauto.
 
  Case "x2 steps".
   inverts H1. inverts H2.
   inverts H1.
-  eapply EVLamApp.
-   apply H4.
-   auto.
-   eauto. 
-   eapply IHSTEP; eauto.
-   eauto.
+  eapply EVLamApp; eauto.
 Qed.
 
