proof/Simple/Progress.v
@@ -18,9 +18,7 @@ Proof.
   subst. inverts H.
 
  Case "XLam".
-  left. clear IHTYPE. subst. apply TYLam in H.
-  apply type_check_empty_tyenv_is_closed in H.
-  eauto.
+  left. subst. eauto. 
 
  Case "XApp".
   right. 
@@ -31,9 +29,10 @@ Proof.
   SCase "value x1".
    destruct IHTYPE2.
    SSCase "value x2".
-    inverts H1.
-    exists (subst x2 x).
-    apply ESLamApp. auto.
+    inverts H1. inverts H3.
+     inverts H4. false.
+     exists (subst x2 x0).
+     apply ESLamApp. auto.
    SSCase "x2 steps".
     destruct H2 as [x2'].
     exists (XApp x1 x2'). auto.
@@ -44,14 +43,3 @@ Proof.
 Qed.
 
 
-(* This doesn't work directly as we have nothing to induct over *)
-(*
-Theorem progress_steps
- :  forall x1 t1 
- ,  TYPE Empty x1 t1
- -> exists v1, value v1 /\ STEPS x1 v1.
-Proof.
- intros.
- apply progress in H.
-Qed.
-*)
